lakefile.lean
@@ -2,10 +2,10 @@ import Lake
 open Lake DSL
 
 package «lean-sts» where
-  moreLeanArgs := #[s!"--load-dynlib={nameToSharedLib "c++"}.1"]
   -- add package configuration options here
-  moreLinkArgs := #["-lstdc++"]
-  moreGlobalServerArgs := #[s!"--load-dynlib={nameToSharedLib "c++"}.1"]
+  -- moreLeanArgs := #[s!"--load-dynlib={nameToSharedLib "c++"}.1"]
+  -- moreLinkArgs := #["-lstdc++"]
+  -- moreGlobalServerArgs := #[s!"--load-dynlib={nameToSharedLib "c++"}.1"]
 
 lean_lib «LeanSts» where
   -- add library configuration options here
@@ -16,7 +16,7 @@ lean_lib «Examples» where
 -- lean-smt includes mathlib
 -- require mathlib from git "https://github.com/leanprover-community/mathlib4.git" @ "v4.4.0"
 
-require auto from git "https://github.com/leanprover-community/lean-auto.git" @ "main"
+require auto from git "https://github.com/dranov/lean-auto.git" @ "dranov"
 require mathlib from git "https://github.com/leanprover-community/mathlib4.git" @ "v4.6.0-rc1"
 
 @[default_target]
